Defined selection sort using fuel recursion and Bove-Capretta. Rewrote merge using fix-in-fix technique. Defined mergesort using Bove-Capretta.

Mergesort.v
@@ -1,8 +1,23 @@
-(* Mergesort *)
+Require Import Sort.
 
-(*Require Import List.
-Import ListNotations.*)
+Fixpoint merge (A : LinDec) (l1 : list A) {struct l1} : list A -> list A :=
+    fix f (l2 : list A) {struct l2} : list A :=
+    match l1, l2 with
+        | [], _ => l2
+        | _, [] => l1
+        | h1 :: t1, h2 :: t2 =>
+            if @leq_total_dec A h1 h2
+            then h1 :: merge A t1 l2
+            else h2 :: f t2
+    end.
 
+(*Theorem merge_eq1 : forall (A : LinDec) (h1 h2 : A) (t1 t2 : list A),
+  @leq A h1 h2 -> merge A (h1 :: t1) (h2 :: t2) = h1 :: merge A t1 (h2 :: t2).
+Proof.
+  intros. simpl. Check leq_total_dec. Print sumbool.*)
+
+
+Eval compute in merge natle [1; 2; 3] [4; 5; 6].
 
 Fixpoint merge' {A : LinDec} (n : nat) (l1 l2 : list A) : option (list A) :=
 match n, l1, l2 with
@@ -21,6 +36,36 @@ match n, l1, l2 with
         end
 end.
 
+Eval compute in merge' 10 [1; 2; 3] [4; 5; 6].
+
+Hint Constructors sorted.
+
+Theorem merge_sorted : forall (A : LinDec) (l1 l2 : list A),
+    sorted A l1 -> sorted A l2 -> sorted A (merge A l1 l2).
+Proof.
+  intros A l1 l2 H. generalize dependent l2.
+  induction H.
+    destruct l2; auto.
+    induction 1.
+      simpl. auto.
+      simpl. destruct (leq_total_dec x x0); auto.
+      simpl in *. destruct (leq_total_dec x x0); auto.
+        destruct (leq_total_dec x y); auto.
+    induction 1.
+      simpl. auto.
+      specialize (IHsorted _ (sorted1 A x0)). simpl in *.
+        destruct (leq_total_dec x x0); auto.
+          destruct (leq_total_dec y x0); simpl; auto.
+      simpl. destruct (leq_total_dec x x0).
+        
+
+assert (sorted A (y0 :: l0) -> sorted A (merge A (y :: l) (y0 :: l0))).
+        intro. clear H3.
+Abort. 
+          
+        
+        
+
 Theorem merge_sorted' : forall (A : LinDec) (n : nat) (l1 l2 l : list A),
     sorted A l1 -> sorted A l2 -> merge' n l1 l2 = Some l ->
     sorted A l.
@@ -32,7 +77,7 @@ Proof.
         destruct n; inversion H2; constructor; auto.
         destruct n, l2; inversion H2. constructor. auto.
   
-
+Abort. (*
   induction n as [| n']; intros.
     inversion H1.
     induction H.
@@ -40,22 +85,20 @@ Proof.
       apply (IHn' [x] l2). constructor. auto. rewrite <- H1. destruct n'.
         simpl in *. destruct l2. inversion H1.
   induction 1. Print merge_func.
-Abort.
+Abort.*)
 
-Program Fixpoint merge (A : LinDec) (l1 l2 : list A)
+Program Fixpoint merge2 (A : LinDec) (l1 l2 : list A)
     {measure (length l1 + length l2)} : list A :=
 match l1, l2 with
     | nil, _ => l2
     | _, nil => l1
     | h :: t, h' :: t' => if leq_dec h h'
-        then h :: (merge A t (h' :: t'))
-        else h' :: (merge A (h :: t) t')
+        then h :: (merge2 A t l2)
+        else h' :: (merge2 A l1 t')
 end.
 Next Obligation. simpl; omega. Defined.
 
-Eval compute in merge natle [1; 2; 3] [4; 5; 6].
-
-(*Eval compute in merge natle (5 :: _) (6 :: _).*)
+Eval compute in merge2 natle [1; 2; 3] [4; 5; 6].
 
 (*Theorem merge_eq : forall (A : LinDec) (l1 l2 : list A),
     merge A l1 l2 = match l1, l2 with
@@ -111,7 +154,9 @@ end.
 Theorem take_length : forall (A : Type) (n : nat) (l : list A),
     length (take n l) <= length l.
 Proof.
-  induction n as [| n']; destruct l; simpl; intros; auto; omega.
+  induction n as [| n']; destruct l; simpl; intros; auto.
+    omega.
+    apply le_n_S. apply IHn'.
 Qed.
 
 Theorem take_length2 : forall (A : Type) (n : nat) (l : list A),
@@ -137,6 +182,9 @@ Proof.
     contradiction H0. trivial.
     unfold lt. apply le_n_S. apply drop_length.
 Qed.
+
+Require Import Arith.
+Require Import Div2.
 
 Program Fixpoint mergeSort (A : LinDec) (l : list A) 
     {measure (length l)} : list A :=
@@ -167,5 +215,39 @@ match l with
     | l1 :: l2 :: t => merge A l1 l2 :: aux A t
 end.
 
-Eval compute in merge natle (qs natle [5; 2; 8]) (qs natle [6; 4; 9]).
+(*Eval compute in merge natle (qs natle [5; 2; 8]) (qs natle [6; 4; 9]).*)
 Eval compute in aux natle [[5; 2; 8]; [1; 4; 9]].
+
+(* Mergesort using Bove-Capretta *)
+
+Inductive msDom' (A : LinDec) : list A -> Type :=
+    | msDom_base : msDom' A []
+    | msDom_base' : forall x : A, msDom' A [x]
+    | msDom_rec : forall l : list A,
+        msDom' A (take (div2 (length l)) l) ->
+        msDom' A (drop (div2 (length l)) l) -> msDom' A l.
+
+Fixpoint ms_aux (A : LinDec) (l : list A) (dom : msDom' A l) : list A :=
+match dom with
+    | msDom_base => []
+    | msDom_base' x => [x]
+    | msDom_rec l dom1 dom2 =>
+        let l1 := ms_aux A _ dom1 in
+        let l2 := ms_aux A _ dom2 in merge A l1 l2
+end.
+
+Theorem msDom_all : forall (A : LinDec) (l : list A), msDom' A l.
+Proof.
+  intro.
+  apply well_founded_induction_type with (fun l1 l2 => length l1 < length l2).
+    eapply well_founded_lt_compat. eauto.
+    intros l ms. destruct l as [| h [| h' t]]; constructor.
+      
+      apply ms. apply take_length2. apply lt_div2. simpl. omega.
+      apply ms. apply drop_length2. simpl. omega. inversion 1.
+Defined.
+
+Definition ms {A : LinDec} (l : list A) : list A :=
+    ms_aux A l (msDom_all A l).
+
+Eval compute in @ms natle testl.
