SelectionSort.v
@@ -57,6 +57,16 @@ Proof.
       simpl. apply lt_n_S. apply IHt. assumption.
 Defined.
 
+Lemma remove_once_min_lengthOrder : forall (A : LinDecMin) (l : list A),
+    l <> [] -> lengthOrder (remove_once (min' A l) l) l.
+Proof.
+  red; intros. apply remove_once_length2. apply min'_In. assumption.
+Defined.
+
+Lemma cons_not_nil : forall (A : Type) (h : A) (t : list A),
+    h :: t <> [].
+Proof. inversion 1. Defined.
+
 (* Selection sort using program fixpoint *)
 Program Fixpoint selectionSort (A : LinDecMin) (l : list A)
     {measure (length l)} : list A :=
@@ -68,6 +78,127 @@ end.
 Next Obligation. apply remove_once_length2. apply min'_In. auto. Qed.
 
 Eval compute in selectionSort natle_min testl.
+
+(* Selection sort using fuel recursion. *)
+Fixpoint selectionSortFuel {A : LinDecMin} (n : nat) (l : list A)
+    : option (list A) :=
+match n with
+    | 0 => None
+    | S n' =>
+        match l with
+            | [] => Some []
+            | _ => let m := min' A l in
+                match selectionSortFuel n' (remove_once m l) with
+                    | None => None
+                    | Some l' => Some (m :: l')
+                end
+            end
+end.
+
+Eval compute in selectionSortFuel 3 [2; 1].
+
+Lemma wut : forall (A : LinDecMin) (n : nat) (h : A) (t : list A),
+    selectionSortFuel (S n) (h :: t) =
+        (*let m := min' A (h :: t) in*)
+        match selectionSortFuel n (remove_once (min' A (h :: t)) (h :: t)) with
+            | None => None
+            | Some l => Some (min' A (h :: t) :: l)
+        end.
+Proof.
+  intros. reflexivity.
+Qed.
+
+Lemma remove_once_length3 : forall (A : LinDecMin) (x : A) (l : list A),
+    In x l -> S (length (remove_once x l)) = length l.
+Proof.
+  induction l as [| h t]; simpl.
+    inversion 1.
+    destruct 1; destruct (x =? h); simpl; auto.
+      subst. intuition.
+Defined.
+
+Theorem selectionSortFuel_extract : forall (A : LinDecMin) (l : list A),
+    {l' : list A | selectionSortFuel (S (length l)) l = Some l'}.
+Proof.
+  intro. apply (Fix (@lengthOrder_wf A)). intros l H.
+  destruct l as [| h t]; intros.
+    simpl. exists []. trivial.
+    pose (m := min' A (h :: t)). pose (r := remove_once m (h :: t)).
+      destruct (H r).
+        unfold r. apply remove_once_min_lengthOrder. inversion 1.
+ 	exists (min' A (h :: t) :: x). rewrite wut. fold m. fold r.
+          replace (length (h :: t)) with (S (length r)).
+            rewrite e. reflexivity.
+            unfold r. rewrite remove_once_length3.
+              trivial.
+              unfold m. apply min'_In. inversion 1.
+Defined.
+
+Theorem ssfuel_none : forall (A : LinDecMin) (l : list A),
+    selectionSortFuel (S (length l)) l <> None.
+Proof.
+  unfold not; intros.
+  pose (H' := selectionSortFuel_extract A l).
+  destruct H'. rewrite e in H. inversion H.
+Defined.
+
+Definition selectionSort4 {A : LinDecMin} (l : list A) : list A :=
+    proj1_sig (selectionSortFuel_extract A l).
+
+(* TODO : Eval compute in selectionSort4 [1]. *)
+
+Definition selectionSort4' {A : LinDecMin} (l : list A) : list A.
+Proof.
+  case_eq (selectionSortFuel (S (length l)) l); intros.
+    exact l0.
+    apply ssfuel_none in H. destruct H.
+Defined.
+
+Eval compute in selectionSort4' [3; 1; 2; 3].
+
+Fixpoint ssfuel2 {A : LinDecMin} (n : nat) (l : list A) : list A :=
+match n, l with
+    | 0, _ => []
+    | _, [] => []
+    | S n', _ => let m := min' A l in
+        m :: ssfuel2 n' (remove_once m l)
+end.
+
+Eval compute in ssfuel2 100 testl.
+
+(* Selection sort using well-founded recursion *)
+
+Definition selectionSort3 {A : LinDecMin} : list A -> list A.
+Proof.
+  apply (Fix (@lengthOrder_wf A)). intros l selectionSort.
+  destruct l as [| h t].
+    exact [].
+    pose (m := min' A (h :: t)). pose (r := remove_once m (h :: t)).
+      pose (p := remove_once_min_lengthOrder A (h :: t) (cons_not_nil _ h t)).
+      exact (m :: selectionSort r p).
+      (*exact r.*)
+Defined.
+
+Print Assumptions selectionSort3.
+
+Transparent selectionSort3.
+
+(* TODO : Eval compute in selectionSort3 [2; 1].
+
+Definition selectionSort3' {A : LinDecMin}
+    : list A -> list A.
+refine (Fix (@lengthOrder_wf A) _
+(fun (l : list A) (ss : forall l' : list A, lengthOrder l' l -> list A) =>
+    match l with
+        | [] => []
+        | h :: t => let m := min' A (h :: t) in m :: ss (remove_once m (h :: t)) _
+    end)).
+Proof.
+  red. apply remove_once_length2. apply min'_In.
+*)
+
+
+
 
 (* Selection sort using Bove-Capretta *)
 
@@ -83,75 +214,21 @@ match p with
     | ssDomRec l p => min' A l :: selectionSort2' p
 end.
 
-(*Theorem ssDom_all : forall (A : LinDecMin) (l : list A), ssDom l.
+Theorem ssDom_all : forall (A : LinDecMin) (l : list A), ssDom l.
 Proof.
+  intro.
+  apply well_founded_induction_type with (fun l1 l2 => length l1 < length l2).
+    eapply well_founded_lt_compat. eauto.
+    intros l ss. destruct l as [| h t]; constructor.
+      apply ss. apply remove_once_length2. apply min'_In. inversion 1.
+Defined. (*
   induction l as [| h t].
     constructor.
     apply ssDomRec. simpl. destruct t.
       dec. constructor.
-      
-Qed.
+Abort.*)
 
 Fixpoint selectionSort2 {A : LinDecMin} (l : list A) : list A :=
-match l with
-    | [] => []
-    | _ => let m := min l in selectionSort2'*)
+    selectionSort2' (ssDom_all A l).
 
-(* Selection sort using well-founded recursion *)
-
-Definition lengthOrder {A : Type} (l1 l2 : list A) : Prop :=
-    length l1 < length l2.
-
-Lemma lengthOrder_wf' : forall (A : Type) (n : nat) (l : list A),
-    length l <= n -> Acc lengthOrder l.
-Proof.
-  induction n as [| n'].
-    inversion 1. destruct l; inversion H1. constructor. inversion 1.
-    intros. destruct l.
-      constructor. inversion 1.
-      simpl in H. constructor. intros. apply IHn'.
-        unfold lengthOrder in H0. simpl in H0. unfold lt in H0.
-        apply le_S_n in H. apply le_S_n in H0. eapply Le.le_trans; eauto.
-Defined.
-
-Theorem lengthOrder_wf : forall (A : Type),
-    well_founded (@lengthOrder A).
-Proof.
-  red. intros A l. apply lengthOrder_wf' with (length l). trivial.
-Defined.
-
-Lemma remove_once_min_lengthOrder : forall (A : LinDecMin) (l : list A),
-    l <> [] -> lengthOrder (remove_once (min' A l) l) l.
-Proof.
-  red; intros. apply remove_once_length2. apply min'_In. assumption.
-Defined.
-
-Lemma cons_not_nil : forall (A : Type) (h : A) (t : list A),
-    h :: t <> [].
-Proof. inversion 1. Defined.
-
-Definition selectionSort3 {A : LinDecMin} : list A -> list A.
-Proof.
-  apply (Fix (@lengthOrder_wf A)). intros l selectionSort.
-  destruct l as [| h t].
-    exact [].
-    pose (m := min' A (h :: t)). pose (r := remove_once m (h :: t)).
-      pose (p := remove_once_min_lengthOrder A (h :: t) (cons_not_nil _ h t)).
-      exact (m :: selectionSort r p).
-      (*exact r.*)
-Defined.
-
-Eval compute in selectionSort3 [2; 1].
-
-Definition selectionSort3' {A : LinDecMin}
-    : list A -> list A.
-refine (Fix (@lengthOrder_wf A) _
-(fun (l : list A) (ss : forall l' : list A, lengthOrder l' l -> list A) =>
-    match l with
-        | [] => []
-        | h :: t => let m := min' A (h :: t) in m :: ss (remove_once m (h :: t)) _
-    end)).
-Proof.
-  red. apply remove_once_length2. apply min'_In.
-
-
+Eval compute in selectionSort2 testl.
