make_makefile.sh
@@ -1,0 +1,3 @@
+#!/bin/sh
+
+coq_makefile -R "." Rand -o makefile *v
