rebuild.sh
@@ -1,0 +1,5 @@
+#!/bin/sh
+
+make clean
+./make_makefile
+make
